Using Index type, testing if I can push

all_MIS_Refine.v
@@ -5,7 +5,13 @@ Require Import wf_combinators.
 Require Import Wellfounded.
 Require Import Relations.
 Require Import List. 
-
+Require Import Omega.
+Require Import index.
+(* Require Import Fin. *)
+Definition iN (N : nat) :=  Ix N.
+Require Import Coq.extraction.ExtrHaskellString.
+Extraction Language Haskell.
+Extract Inductive sumbool => "Prelude.Bool" ["Prelude.True" "Prelude.False"].
 Section RefineMIS.
   (** Let's set up the environment we need to apply queueMIS **)
 
@@ -14,8 +20,9 @@ Section RefineMIS.
 
   (* The list we iterate over is composed of ordered pairs of (N,S)
       where S is a maximal independent set of a graph of size N *)
-
-  Notation A := (nat*(list nat))%type.
+  (* Left part of pair is Index type to allow for the relation over 
+     A to be total *)
+  Notation A := (iN (S |V|) *(list nat))%type.
 
   (* The output should store MISs of the input graph (as a list of list of nats) *)
   Notation B := (list (list nat)).
@@ -23,40 +30,134 @@ Section RefineMIS.
   (* At each step of the function the head of the list is removed
       and replaced with a new list of MISs s.t. N is larger by one,
       but no larger than the vertices of G. *)
-  Definition R : A -> A -> Prop :=
-    LeftProdRel nat (list nat) (fun n m => m < n <= |V|).
 
-  (* Elements are equivalent with respect to R if their
-      fist projections are identical *)
-  Definition Eqa (a1 a2 : A) : Prop := fst a1 = fst a2.
-
-  Lemma R_wf : well_founded R.
+(* Coercion nat_of_fin' (N:nat) (x:iN N) : nat := proj1_sig (Fin.to_nat x). *)
+  Definition iXToNat (x : iN (S |V|)) : nat.
   Proof.
-    apply LeftProdRel_wf.
-    apply PeanoNat.Nat.gt_wf.
-  Qed.
-  
+    destruct x.
+    exact i.
+  Defined.
+
+  Definition R : A -> A -> Prop :=
+    LeftProdRel (iN (S |V|)) (list nat)
+                (fun n m => iXToNat n < iXToNat m <= |V|).
+(* ltof (iN (|V|)) iXToNat n m). *)
+
+Ltac solve_by_inverts n :=
+  match goal with
+  | H : _ /\ _ |- _ => destruct H
+  | |- _ /\ _ => split
+  | H : ?T |- _ => 
+  match type of T with Prop =>
+    solve [ 
+      inversion H; try reflexivity; eauto;
+      match n with S (S (?n')) => subst; solve_by_inverts (n') end ]
+  end end;
+   intros; eauto; solve_by_inverts (n-1).
+
+Ltac si :=
+  try solve_by_inverts 3; eauto.
+
+
+Set Implicit Arguments.
+
+Definition Eqa (a1 a2 : (iN (S|V|) * list nat)) : Prop := fst a1 = fst a2.
+
+Lemma R_wf : well_founded R.
+  apply LeftProdRel_wf.
+  apply well_founded_lt_compat with (f := iXToNat).
+  intros.
+  inversion H.
+  auto.
+Qed.
+
   Lemma R_trans : forall a1 a2 a3, R a1 a2 -> R a2 a3 -> R a1 a3.
   Proof.
-   
-  Admitted.
+    unfold R.
+    unfold ltof.
+    intros.
+    inversion H.
+    subst.
+    inversion H0.
+    subst.
+    constructor.
+    omega.
+  Qed.
 
   Lemma Eqa_eq : equivalence _ Eqa.
   Proof.
-
-  Admitted.
-
-  Lemma R_total : (forall a1 a2 : A, {R a1 a2} + {Eqa a1 a2} + {R a2 a1}).
-  Proof.
-
-  Admitted.
+    constructor; 
+      [constructor; reflexivity |  | ];
+      intros; try omega.
+    {
+      unfold transitive.
+      intros.
+      inversion H.
+      -
+        inversion H0.
+        *
+          unfold Eqa.
+          rewrite H2,H3.
+          auto.
+    }
+    unfold symmetric.
+    intros.
+    inversion H.
+    unfold Eqa.
+    rewrite H1.
+    reflexivity.
+  Qed.
 
   Lemma R_irref : (forall a1 a2 : A, R a1 a2 -> ~ Eqa a1 a2).
   Proof.
+    unfold R,Eqa.
+    unfold ltof.
+    intros.
+    destruct a1,a2.
+    simpl in *.
+    inversion H.
+    subst.
+    simpl in H0.
+    destruct i, i0.
+    intros Hnot.
+    rewrite Hnot in H0.
+    omega.
+  Qed.
 
-  Admitted.
+Require Import ProofIrrelevance.
+
+  Lemma R_total : (forall a1 a2 : A, {R a1 a2} + {Eqa a1 a2} + {R a2 a1}).
+  Proof.
+    intros.
+    unfold R.
+    unfold ltof.
+    unfold Eqa.
+    destruct a1,a2.
+    destruct i,i0.
+    destruct (lt_eq_lt_dec i i0).
+    destruct s.
+    +
+      left.
+      left.
+      constructor; auto.
+      simpl.
+      omega.
+    +
+      left.
+      right.
+      simpl.
+      subst.
+      f_equal.
+      apply proof_irrelevance.
+    +
+      right.
+      constructor.
+      simpl.
+      omega.
+  Defined.
+
   Definition Accum (a : A) (acc : B) : B :=
-    if Nat.eqb (fst a) |V| then (snd a)::acc else acc.
+    if Nat.eqb (iXToNat (fst a)) |V| then (snd a)::acc else acc.
     
 
   (** This should be performing this step of the
@@ -80,30 +181,57 @@ Check mkCandidateSets. About LiftGraph.
         G_s - The next subgraph we need to build an MIS for.
                ^--- This means that newest vertex in G_s is graphSize.
     *)
-  Definition stepCandSet (mis : A) : list A :=
+
+(* function over nats that will be refined to use index type
+   was having trouble with dependent case analysis when using 
+   Index type. *)
+Definition stepCandSet' (mis : nat * list nat) : list (nat * list nat) :=
     let (graphSize, cand) := mis in
     let G_graphSize := LiftGraph graphSize G in    
     let G_s := (LiftGraph (S graphSize) G) in
-      if (Nat.eqb graphSize |V|) (* Is this an MIS of the whole graph G? Then drop it*)
-        then nil
-      else if independent_lGraph G_s (graphSize::cand)
-        then (S graphSize, (cons graphSize cand))::nil
+    match (Nat.eqb graphSize |V|) with
+      (* if (Nat.eqb graphSizeN |V|) *) (* Is this an MIS of the whole graph G? Then drop it*)
+      |true => nil 
+                 (* then nil *)
+      |false => 
+      if independent_lGraph G_s (graphSize::cand)
+        then (graphSize, (cons graphSize cand))::nil
       else if isMIS G_s (graphSize :: (rmvNeighbors graphSize G_s cand))
         then if LFMIS_dec G_graphSize (rmvNeighbors graphSize G_s cand) cand
-          then  (S graphSize, (graphSize :: (rmvNeighbors graphSize G_s cand)))::
-                (S graphSize, cand)::
+          then  ((S graphSize), (graphSize :: (rmvNeighbors graphSize G_s cand)))::
+                ((S graphSize), cand)::
                 nil
-          else (S graphSize, cand)::nil
-      else (S graphSize, cand)::nil.
+          else ((S graphSize), cand)::nil
+           else ((S graphSize), cand)::nil
+    end.
 
-  Lemma stepCandSet_desc : forall a a' : A, In a' (stepCandSet a) -> R a' a.
-  Proof.
-
+Lemma stepCand_spec : forall n l,
+    n < S |V| -> (forall l' m,
+    In (m, l') (stepCandSet' l) -> 
+    m < S |V|).
+Proof.
   Admitted.
+
+Definition stepCandSet (mis : A) : list A.
+  destruct mis.
+  destruct i.
+  
+  (* destruct (lex_order.list_in_dec (S i) ). *)
+  (* apply stepCand_spec1 in pf.   *)
+          
+Lemma stepCandSet_desc : forall a a' : A, In a' (stepCandSet a) -> R a' a.
+  Proof.
+  Admitted.
+
 
   Definition queueMIS :=
     IterQueueWithAccum A B R Eqa R_wf R_trans Eqa_eq R_total R_irref
       Accum stepCandSet stepCandSet_desc. 
+
+End RefineMIS.
+
+Extraction queueMIS.
+  Extraction
 
   Lemma queueMIS_EQ_PrintMIS : snd (queueMIS ((0, nil)::nil, nil)) = PrintMIS G.
   Proof.
@@ -114,3 +242,6 @@ Check mkCandidateSets. About LiftGraph.
     IterStackWithAccum A B R R_wf Accum stepCandSet stepCandSet_desc.
 
 End RefineMIS.
+
+
+
